{
 "cells": [
  {
   "cell_type": "markdown",
   "id": "66531668-7e49-4751-a55f-27eadda84739",
   "metadata": {},
   "source": [
    "# Unit 2: Complex Exponentials and ODEs - Part b: The Complex Exponential Function (WIP)"
   ]
  },
  {
   "cell_type": "markdown",
   "id": "b19b546c-97f4-4dec-8b6c-9f620ca77935",
   "metadata": {},
   "source": [
    "## 2. The complex exponential function\n",
    "\n",
    "### In the last lecture, we used Euler's formula to write a complex number $a+bi$ in polar form $r e^{i\\theta}$. In solving ODEs, it is going to be useful to define the complex exponential $e^z$ for any complex number $z=a+ib$.\n",
    "\n",
    "### Moreover:\n",
    "\n",
    "### ***Definition 2.1***\n",
    "### For any complex number $z$, the complex function $e^{zt}$ of a real variable $t$ is defined as the solution to the initial value problem\n",
    "## $$ \\frac{d}{dt} e{zt} = z e^{zt},\\quad e^{z 0} = 1 $$\n",
    " \n",
    "### ***Properties of $e^{it}$***\n",
    "### For every real number $t$,\n",
    "### 1. $e^{it} = \\cos(t) + i \\sin(t)$ (***Euler's formula***),\n",
    "### 2. $e^{-it} = \\overline{e^{it}} = \\cos(t) - i \\sin(t)$,\n",
    "### 3. $|e^{it}| = 1$.\n",
    "\n",
    "### 1. (This is the justification from the previous lecture.) The calculation\n",
    "## $$ \\begin{array} {rcl} \\displaystyle \\frac{d}{dt} (\\cos(t + i \\sin(t)) & = & \\displaystyle -\\sin(t) + i \\cos(t) \\\\ \\, & = & \\displaystyle i(\\cos(t) + i \\sin(t)) \\end{array} $$\t\t \t \n",
    "\n",
    "### shows that the function $F(t) = \\cos(t) + i \\sin(t)$ is the solution to the DE with initial condition\n",
    "## $$ \\dot{F}(t) = i F(t),\\quad F(0) = 1 $$\n",
    " \n",
    "### But by definition $G(t) = e^{it}$ also satisfies\n",
    "## $$ \\dot{G}(t) = i G(t),\\quad G(0) = 1 $$\n",
    " \n",
    "### The Existence and Uniqueness theorem for (first order) differential equations applies to complex-valued functions of a real variable. The uniqueness theorem tells us that $F(t) = G(t)$, or\n",
    "## $$ e^{it} = \\cos(t) + i \\sin(t) $$\n",
    " \n",
    "### The proof of 2. and 3. follow using 1.\n",
    "\n",
    "### ***Properties of the complex exponential***\n",
    "### 1. $e^{a+ib} = e^a(\\cos(b)+i\\sin(b))$ for all real numbers $a$ and $b$ (***Generalized Euler equation***).\n",
    "### 2. $e^{z+w} = e^z e^w$ for all complex numbers $z$ and $w$.\n",
    "### 3. $(e^z)^n = e^{nz}$ for every complex number $z$ and integer $n$.\n",
    "### - The $n=0$ case says $(e^z)^0 = e^{0+i 0} = \\cos(0)+i\\sin(0) = 1$.\n",
    "### - The $n=-1$ case says $\\displaystyle \\frac{1}{e^z} = (e^z)^{-1} = e^{-z}$.\n",
    "\n",
    "### ***Taylor series***\n",
    "### The Taylor series for $e^z$ is given by\n",
    "## $$ e^z = 1 + z + \\frac{z^2}{2!} + \\frac{z^3}{3!} + \\cdots $$\n",
    "### This formula can be deduced by multiplying $z$ by $t$, which gives\n",
    "## $$ e^{zt} = 1 + zt + \\frac{(zt)^2}{2!} + \\frac{(zt)^3}{3!} + \\cdots $$\n",
    "### and showing that the right hand side satisfies the initial value problem $\\dot{F} = zF,\\, F(0) = 1$. Uniqueness guarantees that the two sides are then equal. By setting $t=1$, the original statement is shown.\n",
    "\n",
    "### ***Remark 2.2***\n",
    "### Some books use the ***generalized Euler equation*** or the ***Taylor series for*** $e^z$ as the ***definition*** of the complex exponential function. The definition we gave in terms of the initial value problem $\\displaystyle \\frac{d}{dt}e^{zt} = z e^{zt}$ and $e^{z 0} = 1$ focuses on what makes the function useful.\n",
    "\n",
    "### ***Proof of the properties***\n",
    "### The proofs of these facts are similar to the proof of Euler's formula above.\n",
    "### 1. We show that $e^{a+ib} = e^a e^{ib} = e^a (\\cos(b)+i\\sin(b))$ by showing that $e^{(a+ib)t} = e^{at} (\\cos(bt) + i\\sin(bt))$ for real numbers.\n",
    "## $$ \\begin{array} {rcl} \\displaystyle \\frac{d}{dt} e^{at}(\\cos(bt) + i \\sin(bt)) & = & \\displaystyle a e^{at}(\\cos(bt) + i \\sin(bt)) + e^{at}(-b\\sin(bt) + ib\\cos(bt)) \\\\ \\, & = & \\displaystyle a e^{at} (\\cos(bt) + i\\sin(bt)) + e^{at} i b (\\cos(bt) + i\\sin(bt)) \\\\ \\, & = & \\displaystyle (a+ib)e^{at}(\\cos(bt)+i\\sin(bt)) \\end{array} $$\n",
    " \t \t\t \t \n",
    "### This shows that $e^{at}(\\cos(bt) + i\\sin(bt))$ is a solution to the initial value problem\n",
    "## $$ \\dot{F} = (a+ib) F, \\quad F(0) = 1 $$\n",
    " \n",
    "### But $e^{(a+ib)t}$ is a solution to this initial value problem by definition. The Uniqueness theorem for differential equations tells us that for all real values of $t$,\n",
    "## $$ e^{(a+ib)t} = e^{at}(\\cos(bt) + i\\sin(bt)) $$\n",
    " \n",
    "### In particular, this equation is true when $t=1$.\n",
    "\n",
    "### 2. Let $z=a+ib$, and $w={c+id}$, then\n",
    "## $$ \\begin{array} {rcl} e^z e^w & = & e^{a+ib}e^{c+id} \\\\ \\, & = & e^{a}e^{ib}e^{c}e^{id} \\\\ \\, & = & e^{a}e^{c}e{ib}e^{id} \\\\ \\, & = & e^{a+c}e^{ib}e^{id} \\end{array} $$\n",
    " \t \t\t \t \n",
    "### So all we need to show is that $e^{ib}e^{id} = e^{ib+id}$. We know that $e^{bit}$ solves the ODE\n",
    "## $$ \\dot{F} = ib F,\\quad F(0) = 1 $$\n",
    " \n",
    "### Notice that\n",
    "## $$ \\begin{array} {rcl} \\displaystyle \\frac{d}{dt} e^{ibt} e^{idt} & = & ibe^{ibt}e^{idt} + id e^{ibt}e^{idt} \\\\ \\, & = & (ib+id)e^{ibt}e^{idt} \\end{array} $$\t\n",
    " \t \t\t \t \n",
    "### Thus both $e^{ibt}e^{idt}$ and $e^{(ib+id)t}$ solve\n",
    "## $$ \\dot{F} = (ib+id) F, \\quad F(0) = 1 $$\n",
    " \n",
    "### The Uniqueness theorem for differential equations implies that these two functions must be equal for all real values of $t$. In particular, they are equal when $t=1$.\n",
    "\n",
    "### 3. If $n=0$, then this is $1=1$ by definition. If $n>0$,\n",
    "## $$ (e^z)^n = \\overbrace{e^z e^z\\cdots e^z}^{n\\,\\text{copies}} \\stackrel{\\text{item}\\,2\\,\\text{repeatedly}}= \\overbrace{e^{z+z+\\cdots +z}}^{n\\,\\text{copies}} = e^{n z} $$\n",
    " \n",
    "### If $n= -m<0$, then\n",
    "## $$ (e^z)^{-m} = \\frac{1}{(e^z)^{m}} \\stackrel{(\\text{just shown})}= \\frac{1}{e^{mz}} = e^{-m z} $$\n",
    " \n",
    "### since $e^{mz}e^{-mz} = e^{mz+(-mz)} = e^0 = 1$."
   ]
  },
  {
   "cell_type": "markdown",
   "id": "51589642-6f5f-4398-bdd6-cdc5ddf2616e",
   "metadata": {},
   "source": [
    "## 3. Proof of Uniqueness\n",
    "\n",
    "### Previously, we defined the function $e^{at}$ to be the solution to this equation guaranteed by the existence and uniqueness theorem, and then used the equation to establish various properties of the exponential function. In this note, we'll just assume that the solution given by the exponential function exists and prove the uniqueness part of the theorem. The most common proof of existence is not too hard but relies on some advanced Calculus – in particular convergence theorems.\n",
    "\n",
    "### We begin by restating with the most basic version of the existence and uniqueness theorem for first order equations with constant (complex) coefficients.\n",
    "\n",
    "### ***Theorem 3.1***\n",
    "### Let $\\alpha\\in \\mathbb{C}$. Then for a given $x_0\\in\\mathbb{C}$, the initial value problem\n",
    "## $$ \\begin{array} {rcl} x'(t) & = & \\alpha x(t) \\\\ x(0) & = & x_0 \\end{array} $$\n",
    "### has a unique solution given by\n",
    "## $$ x(t) = e^{\\alpha t} x_0 $$\n",
    "### ***Proof of uniqueness***\n",
    "### Suppose that $y(t)$ is any other solution to $y'(t) = \\alpha y(t)$. Define\n",
    "## $$ z(t) = e^{-\\alpha t}y(t) $$\n",
    "### Then,\n",
    "## $$ \\begin{array} {rcl} z'(t) & = & -\\alpha e^{-\\alpha t} y(t) + e^{-\\alpha t}y'(t) \\\\ \\, & = & -\\alpha e^{\\alpha t} y(t) + e^{-\\alpha t} \\alpha y(t) \\\\ \\, & = & 0 \\end{array} $$\n",
    "### where above in the second line we used the equation $y'(t) = \\alpha y(t)$. Since $z'(t) = 0$ we know $z(t)$ is equal to a constant. Using the initial conditions $y(0) = x_0$, we see that $z(0) = x_0$, and thus $z(t) = x_0$ for all $t\\in \\mathbb{R}$. Hence,\n",
    "## $$ x_0 = e^{-\\alpha t} y(t) $$\n",
    " \n",
    "### or in other words, $y(t) = e^{\\alpha t}x_0$, which proves uniqueness. $\\square$\n",
    "\n",
    "### The proof above easily generalizes to\n",
    "\n",
    "### ***Theorem 3.2***\n",
    "### (Uniqueness for an inhomogeneous equation) Let $\\alpha \\in \\mathbb{C}$ and let $q(t)$ be a continuous function on an open time interval $J \\subset \\mathbb{R}$ with $0\\in J$. Then for a given $x_0\\in\\mathbb{C}$, the initial value problem\n",
    "## $$ \\begin{array} {rcl} x'(t) - \\alpha x(t) & = & q(t) \\\\ x(0) & = & x_0 \\end{array} $$\n",
    "### has a unique solution on the interval $J$.\n",
    "\n",
    "### The existence part of the theorem can be proved using, say, the variation of parameters formula. We will prove uniqueness here.\n",
    "\n",
    "### ***Proof of uniqueness***\n",
    "### Suppose there are two solutions $x_1(t)$ and $x_2(t)$. Then $w(t):=x_1(t) - x_2(t)$ solves the homogeneous equation,\n",
    "## $$ \\begin{array} {rcl} w'(t) - \\alpha w(t) & = & 0 \\\\ w(0) & = & 0 \\end{array} $$\n",
    "### Then, we just apply the previous argument to conclude that $w(t) = 0$ is the unique solution to the above, and thus $x_1(t) = x_2(t)$ for all $t\\in J$. $\\square$ "
   ]
  },
  {
   "cell_type": "markdown",
   "id": "3c819e0b-e02c-42fd-8723-723c9326a749",
   "metadata": {},
   "source": []
  }
 ],
 "metadata": {
  "kernelspec": {
   "display_name": "Python 3",
   "language": "python",
   "name": "python3"
  },
  "language_info": {
   "codemirror_mode": {
    "name": "ipython",
    "version": 3
   },
   "file_extension": ".py",
   "mimetype": "text/x-python",
   "name": "python",
   "nbconvert_exporter": "python",
   "pygments_lexer": "ipython3",
   "version": "3.8.8"
  }
 },
 "nbformat": 4,
 "nbformat_minor": 5
}
